test/Flat.fst
@@ -1,6 +1,7 @@
 module Flat
 
 open FStar
+open FStar.HST
 
 type point = {
   x: Int32.t;
@@ -10,9 +11,12 @@ type point = {
 
 let x p = p.x
 
-val main: Int32.t -> FStar.Buffer.buffer (FStar.Buffer.buffer C.char) -> HST.Stl C.int
+val main: Int32.t -> FStar.Buffer.buffer (FStar.Buffer.buffer C.char) ->
+  HST.Stack Int32.t (fun _ -> true) (fun _ _ _ -> true)
 let main argc argv =
+  push_frame ();
   let p = { x = 0l; y = 1l; z = -1l } in
   let foo = FStar.Int32 (p.x +^ p.y +^ p.z) in
   let bar = x ({ x = 0l; y = 1l; z = -1l }) in
+  pop_frame ();
   C.exit_success
