kremlib/C.fsti
@@ -1,5 +1,4 @@
 module C
 
 assume val char: Type0
-assume val int: Type0
-assume val exit_success: int
+assume val exit_success: Int32.t
