test/Inline.fst
@@ -1,23 +1,34 @@
 module Inline
 
 open FStar
+open FStar.HyperStack
 open FStar.HST
 open TestLib
 
-let alloc_and_init ():
-  StackInline (Buffer.buffer Int32.t) (fun _ -> true) (fun _ _ _ -> true) =
-  Buffer.createL [ 0l; 1l; 2l; 3l ]
+let alloc_and_init (i: Int32.t): StackInline (Buffer.buffer Int32.t)
+  (requires (fun h0 -> is_stack_region h0.tip))
+    // JP: why do I have to manually write the hypothesis above?
+  (ensures (fun h0 b h1 ->
+    let open FStar.Buffer in
+    length b = 2 /\
+    (forall (b0: buffer Int32.t). live h0 b0 ==> live h1 b0) /\
+    live h1 b))
+=
+  let open FStar.Int32 in
+  Buffer.createL [ i; i +%^ 1l ]
 
-let alloc_and_init' ():
-  StackInline (Buffer.buffer Int32.t) (fun _ -> true) (fun _ _ _ -> true) =
-  Buffer.createL [ 4l; 5l; 6l; 7l ]
+// JP: couldn't figure out how to define trivial_pre and trivial_post so that I
+// don't have to repeat the [fun _ _ _ ...]
 
 val main: Int32.t -> Buffer.buffer (Buffer.buffer C.char) ->
-  Stack C.int (fun _ -> true) (fun _ _ _ -> true)
+  Stack Int32.t (fun _ -> true) (fun _ _ _ -> true)
 let main argc argv =
+  // JP: found no way to make this work with [with_frame]!
   push_frame ();
-  let buf = alloc_and_init () in
-  let buf': Buffer.buffer Int32.t = alloc_and_init' () in
-  check (Buffer.index buf 2ul) 2l;
+  let buf = alloc_and_init 0l in
+  let buf' = alloc_and_init 2l in
+  // If [alloc_and_init] is compiled as a separate function, then the second
+  // call will override the initial value and the check will fail.
+  check (Buffer.index buf 1ul) 1l;
   pop_frame ();
   C.exit_success
