test/Renaming.fst
@@ -3,7 +3,8 @@ module Renaming
 open TestLib
 open FStar.HST
 
-val f: Int64.t -> Stl unit
+val f: Int64.t ->
+  Stack unit (fun _ -> true) (fun _ _ _ -> true)
 let f msg =
   push_frame ();
   let x = 1l in
@@ -13,7 +14,8 @@ let f msg =
   touch msg;
   pop_frame ()
 
-val main: Int32.t -> FStar.Buffer.buffer (FStar.Buffer.buffer C.char) -> HST.Stl C.int
+val main: Int32.t -> FStar.Buffer.buffer (FStar.Buffer.buffer C.char) ->
+  HST.Stack Int32.t (fun _ -> true) (fun _ _ _ -> true)
 let main argc argv =
   f 0L;
   C.exit_success
